Tests/AxiomAudit.lean
@@ -102,13 +102,13 @@ elab "#assert_axioms " id:ident : command => do
 /-! ## The merkle tree -/
 
 #assert_axioms BtcVerified.Merkle.combine_inj
-#assert_axioms BtcVerified.Merkle.computeRoot_eq_root
 #assert_axioms BtcVerified.Merkle.root_inj_of_length_eq
 #assert_axioms BtcVerified.Merkle.root_inj_of_canonical
 #assert_axioms BtcVerified.Block.merkleCommits
 
 /-! ## Bitcoin Core's ComputeMerkleRoot -/
 
+#assert_axioms BtcVerified.Impl.BitcoinCore.computeRoot_eq_root
 #assert_axioms BtcVerified.Impl.BitcoinCore.computeMerkleRoot_fst
 #assert_axioms BtcVerified.Impl.BitcoinCore.canonical_of_not_mutated
 #assert_axioms BtcVerified.Impl.BitcoinCore.eq_of_computeMerkleRoot_eq_of_not_mutated
